CCsub_CvFacts.v
@@ -5,185 +5,17 @@ Require Import TaktikZ.
 
 Local Ltac hint := idtac.
 
-
-Lemma cv_unique_shrink_head : forall Y B E T C,
-  wf_env ([(Y, B)] ++ E) ->
-  wf_typ_in E T ->
-  cv ([(Y, B)] ++ E) T C ->
-  cv E T C.
-Proof.
- intros*.
- intros HwfE HwfT Hcv.
-
- assert (type T). eapply type_from_wf_typ; eauto.
-
- dependent induction Hcv.
- * assert (X <> Y). {
-     inversion HwfT; subst.
-     assert (X `in` dom E).
-     eapply binds_In. apply H6.
-     inversion HwfE; subst; notin_solve.
-   }
-   apply cv_typ_var with (T := T).
-   unfold binds in H. unfold get in H. simpl in H.
-   destruct (X == Y) eqn:HXY; subst; trivial.
-   easy.
-
-   inversion HwfE; trivial.
-   eapply IHHcv with (Y0 := Y) (B0 := B).
-   inversion HwfT; subst.
-   {
-     pose proof H7.
-     unfold binds in H. unfold binds in H7.
-     simpl in *.
-     destruct (X == Y); subst; try easy.
-     rewrite H in H7; inversion H7; subst.
-     simpl_env in *.
-     eapply wf_typ_from_binds_sub.
-     inversion H0; trivial.
-     apply H3.
-   }
-   trivial.
-   trivial.
-   eapply type_from_wf_typ.
-   eapply wf_typ_from_binds_sub.
-   apply HwfE. apply H.
- * inversion HwfT; subst. constructor; trivial.
-   inversion H; trivial.
-Qed.
-
-Lemma cv_unique_shrink : forall F E T C,
-  wf_env (F ++ E) ->
-  wf_typ_in E T ->
-  cv (F ++ E) T C ->
-  cv E T C.
-Proof with eauto using cv_unique_shrink_head.
-  intros* WfEnv WfTyp H.
-  induction F; try destruct a; simpl_env in *...
-  apply IHF. inversion WfEnv... eapply cv_unique_shrink_head...
-  rewrite_nil_concat.
-  eapply wf_typ_weakening...
-  simpl_env.
-  inversion WfEnv...
-Qed.
-
-Lemma cv_unique : forall E T C1 C2,
-  wf_env E ->
-  wf_typ_in E T ->
-  cv E T C1 ->
-  cv E T C2 ->
-  C1 = C2.
-Proof with eauto*.
- intros E; induction E; intros T; induction T; intros...
- - inversion H1; inversion H2; subst...
- - exfalso. inversion H0.
- - exfalso.
-   inversion H0...
-   inversion H7...
- - inversion H1...
-   inversion H2...
- - inversion H0.
- - destruct a as [Y B].
-   simpl_env in *.
-   destruct (Y == a0); subst...
-   + inversion H2; subst...
-     inversion H1; subst...
-     apply IHE with (T := T)...
-     * inversion H5; trivial.
-     * binds_cases H4; subst; simpl_env in *; try notin_solve...
-       inversion H; trivial.
-     * binds_cases H4; subst; simpl_env in *; try notin_solve...
-       binds_cases H6; subst; simpl_env in *; try notin_solve...
-       inversion H6; subst...
-       eapply cv_unique_shrink_head...
-       inversion H...
-     * binds_cases H4; subst; simpl_env in *; try notin_solve...
-       binds_cases H6; subst; simpl_env in *; try notin_solve...
-       inversion H6; subst...
-       eapply cv_unique_shrink_head...
-       inversion H...
-   + inversion H1; subst...
-     inversion H2; subst...
-     apply IHE with (T := a0)...
-     * inversion H5; trivial.
-     * binds_cases H4; subst; simpl_env in *; try notin_solve...
-     * eapply cv_unique_shrink_head...
-       binds_cases H4.
-       eapply wf_typ_var...
-     * eapply cv_unique_shrink_head...
-       binds_cases H4.
-       eapply wf_typ_var...
-Qed.
-
-
-Lemma cv_weakening_head : forall E F T C,
-  cv E T C ->
-  wf_env (F ++ E) ->
-  cv (F ++ E) T C.
-Proof with eauto using cv_regular.
-  intros E F T C Hcv Wf.
-
-  induction Hcv.
-  - apply cv_typ_var with (T := T)...
-  - apply cv_typ_capt...
-    rewrite_nil_concat.
-    eapply wf_pretyp_weakening...
-    rewrite_nil_concat.
-    eapply wf_cset_weakening...
-Qed.
-
-Lemma cv_weakening : forall E F G T C,
-  cv (G ++ E) T C ->
-  wf_env (G ++ F ++ E) ->
-  cv (G ++ F ++ E) T C.
-Proof with eauto using cv_regular, wf_pretyp_weakening, wf_cset_weakening.
-  intros E F G T C Hcv Hwf.
-
-  dependent induction Hcv.
-  * apply cv_typ_var with (T := T)...
-  * apply cv_typ_capt...
-Qed.
-
-
-Lemma cv_exists_in : forall E T,
-  wf_env E ->
-  wf_typ_in E T ->
-  exists C, cv E T C.
-Proof with eauto.
-  induction E; induction T; intros; try inversion H0; try inversion H; subst...
-  - inversion H5.
-  - simpl_env in *.
-    binds_cases H5.
-    + destruct (a0 == X0).
-      * subst.
-        specialize (IHE T H8 H9) as [C' H'].
-        exists C'.
-        eapply cv_typ_var...
-        apply cv_weakening_head...
-      * assert (wf_typ_in E a0). { inversion H0; subst... }
-        specialize (IHE a0 H8 H2) as [C' H'].
-        exists C'. apply cv_weakening_head...
-    + inversion H3; subst.
-      specialize (IHE T H8 H9) as [C' H'].
-      exists C'. eapply cv_typ_var...
-      apply cv_weakening_head...
-  - simpl_env in *.
-    assert (wf_typ_in E a0). { inversion H0; subst... binds_cases H6... }
-    specialize (IHE a0 H8 H1) as [C' H'].
-    exists C'. apply cv_weakening_head...
-Qed.
-
 Lemma subcapt_weakening : forall E F G C1 C2,
   subcapt (G ++ E) C1 C2 ->
   wf_env (G ++ F ++ E) ->
   subcapt (G ++ F ++ E) C1 C2.
-Proof with eauto using wf_cset_weakening, cv_weakening.
+Proof with eauto using wf_cset_weakening.
   intros * Hsc Hwf.
   remember (G ++ E).
   remember (G ++ F ++ E).
   induction Hsc ; subst...
+  - apply subcapt_universal...
   - apply subcapt_in...
-  - eapply subcapt_var...
   - apply subcapt_set...
     intros ? ?...
 Qed.
@@ -192,10 +24,10 @@ Create HintDb fsetdec.
 
 Hint Extern 1 (_ `in` _) => fsetdec: fsetdec.
 
-Lemma wf_cset_singleton_by_mem : forall E A x xs,
-  wf_cset E A (cset_set xs {}N) ->
+Lemma wf_cset_singleton_by_mem : forall E A x xs b,
+  wf_cset E A (cset_set xs {}N b) ->
   x `in` xs ->
-  wf_cset E A (cset_set (singleton x) {}N).
+  wf_cset E A (cset_set (singleton x) {}N b).
 Proof with eauto with fsetdec.
   intros * Wfxs xIn.
   inversion Wfxs; subst...
@@ -209,12 +41,11 @@ Lemma subcapt_reflexivity : forall E A C,
   subcapt E C C.
 Proof with eauto.
   intros * WfC HSub.
-  inversion WfC; subst. {
-    constructor...
-  }
-  apply subcapt_set...
-  intros y yIn.
-  apply subcapt_in...
+  inversion WfC; subst.
+  constructor...
+  - intros y yIn.
+    apply subcapt_in...
+  - csetdec.
 Qed.
 
 Lemma subcapt_transitivity : forall E C1 C2 C3,
@@ -224,132 +55,52 @@ Lemma subcapt_transitivity : forall E C1 C2 C3,
   subcapt E C1 C3.
 Proof with eauto with fsetdec.
   intros * WfE SC12 SC23.
-  note (wf_cset_in E C3). {
-    constructor...
-  }
-  rename fvars into es.
-  dependent induction SC12.
-  - inversion SC23.
-  - dependent induction SC23.
-    + apply subcapt_in...
-    + rewrite AtomSetFacts.singleton_iff in H1; subst...
-    + apply H3...
-  - eapply subcapt_var with (T := T)...
-  - eapply subcapt_set...
-    intros y yIn...
-Qed.
+  note (wf_cset_in E C3).
 
-Lemma extract_bind_cv_from_var_cv : forall X E U C,
-  binds X (bind_sub U) E ->
-  cv E X C ->
-  cv E U C.
-Proof with eauto using cv_weakening_head.
-  intros *. intros Hbinds Hcv.
-  dependent induction Hcv.
-  unfold binds in H, Hbinds.
-  rewrite Hbinds in H.
-  inversion H...
+  rename fvars into es, univ into u.
+  dependent induction SC12.
+  - inversion SC23; subst.
+    + apply subcapt_universal...
+    + apply subcapt_universal...
+    + assert (u = true) by csetdec; subst.
+      apply subcapt_universal...
+  - dependent induction SC23.
+    + apply subcapt_universal...
+    + rewrite AtomSetFacts.singleton_iff in H1; symmetry in H1; subst...
+    + apply subcapt_universal...
+    + rewrite AtomSetFacts.singleton_iff in H1; symmetry in H1; subst...
+    + rewrite AtomSetFacts.singleton_iff in H1; symmetry in H1; subst...
+    + eauto.
+  - dependent induction SC23.
+    + apply subcapt_universal...
+    + apply subcapt_universal...
+    + assert (u = true) by csetdec; subst.
+      apply subcapt_universal...
+  - eapply subcapt_var with (T := T)...
+  - eapply subcapt_tvar with (T := T)...
+  - eapply subcapt_set...
+    + intros y yIn...
+    + destr_bool.
+      inversion SC23; subst...
+      subst...
 Qed.
 
 (* Subtyping implies subcapturing *)
-Lemma sub_implies_subcapt : forall E A1 A2 S T C D,
+Lemma sub_implies_subcapt : forall E S T,
   sub E S T ->
-  AtomSet.F.Subset A1 (dom E) ->
-  AtomSet.F.Subset A2 (dom E) ->
-  wf_cset E A1 C ->
-  wf_cset E A2 D ->
-  cv E S C ->
-  cv E T D ->
-  subcapt E C D.
+  wf_cset_in E (cv S) ->
+  wf_cset_in E (cv T) ->
+  subcapt E (cv S) (cv T).
 Local Ltac hint ::=
-  eauto using subcapt_reflexivity, cv_weakening_head, extract_bind_cv_from_var_cv.
+  eauto using subcapt_reflexivity.
 Proof with hint.
-  intros *.
-  intros Hsub HssetA1 HssetA2 WfC WfD HcvC HcvD.
+  intros * Hsub WfC WfD.
 
-  induction Hsub; destruct C; destruct D; try solve [inversion HcvC; inversion HcvD; subst; hint].
-  1,2: forwards Eq: cv_unique H H0 HcvC HcvD; inversion Eq...
-Qed.
-
-Lemma cv_narrowing_exists : forall T G Z Q E P C1,
-  sub E P Q ->
-  cv (G ++ [(Z, bind_sub Q)] ++ E) T C1 ->
-  exists C2, cv (G ++ [(Z, bind_sub P)] ++ E) T C2 /\ subcapt (G ++ [(Z, bind_sub P)] ++ E) C2 C1.
-Local Ltac hint ::=
-  eauto using wf_env_narrowing, wf_typ_narrowing, wf_pretyp_narrowing, wf_cset_narrowing.
-Proof with simpl_env; hint.
-  intros* Hsub Hcv.
-  dependent induction Hcv.
-  - destruct (X == Z).
-    + subst.
-      binds_get H.
-      inversion H2; subst.
-      assert (wf_typ_in E Q)...
-      assert (cv E Q CT). {
-        apply (cv_unique_shrink (G ++ [(Z, bind_sub Q)]))...
-      }
-      assert (wf_typ_in E P) as HA...
-      forwards (D & HcvD): cv_exists_in HA...
-      exists D. split.
-      * eapply cv_typ_var...
-        rewrite_env (empty ++ (G ++ [(Z, bind_sub P)]) ++ E).
-        apply cv_weakening...
-      * rewrite_env (empty ++ (G ++ [(Z, bind_sub P)]) ++ E).
-        apply subcapt_weakening...
-        apply sub_implies_subcapt with (S := P) (T := Q) (A1 := dom E) (A2 := dom E)...
-    + assert (binds X (bind_sub T) (G ++ [(Z, bind_sub P)] ++ E)). {
-        binds_cases H.
-        - assert (wf_env (G ++ [(Z, bind_sub P)] ++ E)). {
-            trivial...
-          }
-          apply binds_tail.
-          apply binds_tail.
-          + assumption.
-          + simpl_env in *; trivial.
-          + trivial.
-        - trivial...
-      }
-      forwards (C2 & HcvC2 & HscC2): IHHcv G Z Q E...
-      exists C2. split.
-      * eapply cv_typ_var...
-      * assumption.
-  - exists C.
-    split...
-    + constructor...
-    + forwards: wf_cset_narrowing P H1...
-      eapply subcapt_reflexivity...
-Qed.
-
-Lemma cv_narrowing : forall T G Z Q E P C1 C2,
-  sub E P Q ->
-  cv (G ++ [(Z, bind_sub Q)] ++ E) T C2 ->
-  cv (G ++ [(Z, bind_sub P)] ++ E) T C1 ->
-  subcapt (G ++ [(Z, bind_sub P)] ++ E) C1 C2.
-Proof with eauto.
-  intros.
-  forwards (? & ? & ?): (>> cv_narrowing_exists T G Z Q E P)...
-  assert (x = C1). {
-    apply (cv_unique (G ++ [(Z, bind_sub P)] ++ E) T)...
-  }
-  subst...
-Qed.
-
-Lemma cv_narrowing_typ : forall Q T G x E P C,
-  sub E P Q ->
-  ok (G ++ [(x, bind_typ Q)] ++ E) ->
-  cv (G ++ [(x, bind_typ Q)] ++ E) T C ->
-  cv (G ++ [(x, bind_typ P)] ++ E) T C.
-Local Ltac hint ::=
-  eauto using wf_env_narrowing_typ, wf_typ_narrowing_typ,
-  wf_pretyp_narrowing_typ, wf_cset_narrowing_typ.
-Proof with simpl_env; hint.
-  intros * HSub Ok HCv.
-  dependent induction HCv.
-  - apply cv_typ_var with (T := T)...
-    binds_cases H.
-    + apply binds_tail. apply binds_tail... trivial.
-    + apply binds_head...
-  - constructor...
+  induction Hsub...
+  eapply subcapt_tvar...
+  apply IHHsub...
+  apply cv_wf.
+  forwards: wf_typ_from_binds_sub H...
 Qed.
 
 (** TODO: reorganize the contents of the bottom of this file **)
@@ -362,9 +113,9 @@ Proof with eauto.
   intros H1 H2.
   inversion H1; inversion H2; subst; simpl...
   unfold wf_cset_in in *.
-  replace (NatSet.F.union _ _) with {}N by fnsetdec.
+  unfold cset_union; csetsimpl.
   constructor...
-  unfold allbound_typ in *...
+  unfold allbound in *...
   intros.
   rewrite AtomSetFacts.union_iff in *.
   auto*.
@@ -379,9 +130,9 @@ Proof with eauto*.
   induction HwfC...
 Qed.
 
-Lemma dom_x_subst_away : forall F E f x b,
+Lemma dom_x_subst_away : forall x f b F E,
   wf_env (F ++ [(x, b)] ++ E) ->
-  dom (map f F ++ E) = dom (F ++ [(x, b)] ++ E) `remove` x. 
+  dom (map f F ++ E) = dom (F ++ [(x, b)] ++ E) `remove` x.
 Proof with eauto*.
   intros * Hwf.
   simpl_env in *.
@@ -391,7 +142,6 @@ Proof with eauto*.
   }
   fsetdec.
 Qed.
-
 
 Lemma wf_env_subst_cb : forall Q C x E F,
 wf_env (F ++ [(x, bind_typ Q)] ++ E) ->
@@ -414,50 +164,27 @@ Proof with eauto using wf_typ_subst_cb, wf_cset_extra.
 Qed.
 
 Lemma cset_subst_self : forall C x,
-  subst_cset x C (cset_fvar x) = C.
+  subst_cset x C (`cset_fvar` x) = C.
 Proof.
   intros.
   unfold subst_cset.
-  destruct (cset_references_fvar_dec x x) eqn:EQ.
-  2: {
-    unfold cset_references_fvar_dec, cset_fvar in EQ.
-    rewrite <- AtomSetFacts.not_mem_iff in EQ.
-    exfalso.
-    fsetdec.
-  }
-  unfold cset_remove_fvar, cset_fvar.
-  replace (cset_set _ _) with {}.
-  2: {
-    apply cset_eq_injectivity; [fsetdec|fnsetdec].
-  }
-  destruct C; simpl.
-  - easy.
-  - replace (cset_set _ _) with (cset_set t t0).
-    2: {
-      apply cset_eq_injectivity; [fsetdec|fnsetdec].
-    }
-    easy.
+  csetdec.
 Qed.
 
-Lemma wf_env_strengthening : forall F E,
-  wf_env (F ++ E) ->
-  wf_env E.
+Lemma wf_env_strengthening : forall F E, wf_env (F ++ E) -> wf_env E.
 Proof with eauto.
   induction F...
   intros.
   inversion H; subst...
 Qed.
 
-
-Lemma wf_cset_remove_fvar : forall A E C x,
-  wf_cset E A C ->
-  wf_cset E A (cset_remove_fvar x C).
+Lemma wf_cset_remove_fvar : forall A E C x, wf_cset E A C -> wf_cset E A (C A`\` x).
 Proof with eauto.
   intros.
   unfold wf_cset_in in *.
   induction H; simpl...
   constructor...
-  unfold allbound_typ in *.
+  unfold allbound in *.
   intros.
   apply H.
   fsetdec.
@@ -472,35 +199,34 @@ Lemma wf_cset_subst_cb : forall Q Ap' Ap F E x C D,
   ok (map (subst_cb x D) F ++ E) ->
   wf_cset (map (subst_cb x D) F ++ E) (Ap `remove` x) (subst_cset x D C).
 Proof with simpl_env; eauto*.
-  intros *. intros HwfC HwfEnv HwfD Hsset HApRsnbl Hok.
+  intros * HwfC HwfEnv HwfD Hsset HApRsnbl Hok.
   destruct C.
-  1: { unfold subst_cset; unfold cset_references_fvar_dec... }
-  unfold subst_cset; unfold cset_references_fvar_dec.
-  apply binding_uniq_from_wf_env in HwfEnv as ?.
-  destruct (AtomSet.F.mem x t) eqn:EQ...
+  unfold subst_cset.
+  forwards: binding_uniq_from_wf_env HwfEnv.
+  destruct_set_mem x t...
   - apply wf_cset_union.
     + rewrite_nil_concat.
       apply wf_cset_weakening with (A := Ap'); simpl_env...
-    + unfold cset_remove_fvar; simpl.
-      inversion HwfC; subst.
+    + inversion HwfC; subst.
       constructor...
-      unfold allbound_typ in *.
-      intros.
-      destruct (x0 == x).
-      * exfalso. fsetdec.
-      * assert (x0 `in` t) as HA by fsetdec.
-        specialize (H4 x0 HA) as [T HbindsT].
-        binds_cases HbindsT...
-        exists (subst_ct x D T)...
+      unfold allbound in *.
+      intros y yIn.
+      destruct (y == x).
+      * exfalso; fsetdec.
+      * forwards (T & B): H4 y.
+        1: fsetdec.
+        simpl_env in B.
+        destruct B as [B|B]; binds_cases B...
+        1,2: exists (subst_ct x D T)...
   - inversion HwfC; subst.
-    rewrite <- AtomSetFacts.not_mem_iff in EQ.
     constructor...
-    unfold allbound_typ in *.
-    intros.
-    unshelve epose proof (H4 x0 _) as [T HbindsT]...
-    assert (x0 <> x) by fsetdec.
-    binds_cases HbindsT...
-    exists (subst_ct x D T)...
+    unfold allbound in *.
+    intros y yIn.
+    forwards (T & B): H4 y.
+    1: fsetdec.
+    simpl_env in B.
+    destruct B as [B|B]; binds_cases B...
+    1,2: exists (subst_ct x D T)...
 Qed.
 
 Lemma wf_cset_in_subst_cb : forall Q F E x C D,
@@ -512,7 +238,7 @@ Lemma wf_cset_in_subst_cb : forall Q F E x C D,
 Proof with eauto.
   intros.
   assert (x `notin` (dom F `union` dom E)). {
-    apply binding_uniq_from_wf_env with (b := bind_typ Q)...
+    forwards: binding_uniq_from_wf_env (bind_typ Q)...
   }
   unfold wf_cset_in in *.
   replace (dom (map (subst_cb x D) F ++ E))
@@ -520,62 +246,11 @@ Proof with eauto.
   apply (wf_cset_subst_cb Q (dom E))...
 Qed.
 
-
 Lemma not_in_fv_cset_iff : forall x C,
-  cset_references_fvar_dec x C = false -> x `notin` fv_cset C.
+  x A`mem` C = false -> x `notin` (`cset_fvars` C).
 Proof.
   intros.
-  unfold cset_references_fvar_dec in H.
-  unfold fv_cset.
-  destruct C.
-  - fsetdec.
-  - rewrite AtomSetFacts.not_mem_iff.
-    assumption.
-Qed.
-
-Lemma cv_through_subst_ct : forall F x U E C T D,
-    cv (F ++ [(x, bind_typ U)] ++ E) T C ->
-    cv E U D ->
-    cv (map (subst_cb x D) F ++ E) (subst_ct x D T) (subst_cset x D C).
-Proof with eauto using wf_env_subst_cb, wf_pretyp_subst_cb, wf_typ_subst_cb, wf_cset_in_subst_cb, wf_cset_extra.
-  intros * HcvT HcvU.
-  dependent induction HcvT.
-  - simpl.
-    binds_cases H.
-    + apply wf_typ_from_binds_sub in H as WfT...
-      rewrite_nil_concat.
-      apply cv_weakening; simpl_env...
-      apply cv_unique_shrink in HcvT...
-      2: {
-        assert (wf_env (F ++ [(x, bind_typ U)] ++ E))...
-        rewrite_nil_concat.
-        eapply wf_typ_weakening; simpl_env.
-        - apply WfT.
-        - apply ok_from_wf_env, ok_tail in H1.
-          assumption.
-        - clear_frees. fsetdec.
-        - clear_frees. fsetdec.
-      }
-      apply cv_unique_shrink in HcvT...
-      apply cv_regular in HcvT as Reg.
-      destruct Reg as [_ [_ WfCT]].
-      inversion WfCT; subst.
-      * unfold subst_cset, cset_references_fvar_dec.
-        eapply cv_typ_var...
-      * apply binding_uniq_from_wf_env in H0 as ?.
-        assert (x `notin` fvars) as HA by notin_solve.
-        rewrite AtomSetFacts.not_mem_iff in HA.
-        unfold subst_cset, cset_references_fvar_dec.
-        rewrite HA.
-        eapply cv_typ_var...
-    + assert (binds X (subst_cb x D (bind_sub T)) (map (subst_cb x D) F ++ E))...
-  - simpl.
-    constructor...
-    unfold wf_pretyp_in.
-    erewrite dom_x_subst_away...
-    eapply wf_pretyp_subst_cb...
-    1, 2: simpl_env in *; apply wf_cset_extra...
-    apply (wf_cset_in_subst_cb U)...
+  csetdec.
 Qed.
 
 Lemma wf_env_weaken_head : forall E F,
@@ -591,7 +266,7 @@ Lemma tail_not_in_head : forall (E F : env) x,
   ok (F ++ E) ->
   x `in` dom E ->
   x `notin` dom F.
-Proof. 
+Proof.
   intros * Hok Hx.
   induction F.
   + notin_solve.
@@ -607,102 +282,120 @@ Proof.
     fsetdec.
 Qed.
 
-Lemma wf_typ_in_subst_cb_cv : forall U F E x C T,
+Lemma wf_env_tail : forall F E,
+  wf_env (F ++ E) ->
+  wf_env E.
+Proof with eauto.
+  intros * Hwf.
+  induction F; (trivial || inversion Hwf; subst)...
+Qed.
+
+Hint Resolve wf_env_tail : core.
+
+(* Lemma wf_env_tail2 : forall F x b E, *)
+(*   wf_env (F ++ [(x, b)] ++ E) -> *)
+(*   wf_env E. *)
+(* Proof with eauto. *)
+(*   intros * Hwf. *)
+(*   eauto using wf_env_tail. *)
+(* Qed. *)
+
+Hint Extern 1 (ok (map ?f ?F ++ ?E)) =>
+match goal with
+| H : wf_env (F ++ ?b ++ E) |- _ =>
+  enough (ok (F ++ b ++ E))
+end : core.
+
+Lemma wf_cv_env_bind_typ : forall F x U E,
+  wf_env (F ++ [(x, bind_typ U)] ++ E) ->
+  wf_cset_in E (cv U).
+Proof with eauto.
+  intros * H.
+  apply cv_wf.
+  assert (wf_env ([(x, bind_typ U)] ++ E)) as HA by eauto.
+  inversion HA...
+Qed.
+
+Lemma wf_typ_env_bind_typ : forall F x U E,
+  wf_env (F ++ [(x, bind_typ U)] ++ E) ->
+  wf_typ_in E U.
+Proof with eauto.
+  intros * H.
+  assert (wf_env ([(x, bind_typ U)] ++ E)) as HA by eauto.
+  inversion HA...
+Qed.
+
+Lemma wf_typ_env_bind_sub : forall F x U E,
+  wf_env (F ++ [(x, bind_sub U)] ++ E) ->
+  wf_typ_in E U.
+Proof with eauto.
+  intros * H.
+  assert (wf_env ([(x, bind_sub U)] ++ E)) as HA by eauto.
+  inversion HA...
+Qed.
+
+Hint Resolve wf_cv_env_bind_typ : core.
+Hint Resolve wf_typ_env_bind_typ : core.
+Hint Resolve wf_typ_env_bind_sub : core.
+
+Lemma wf_typ_in_subst_cb_cv : forall U F E x T,
   wf_env (F ++ [(x, bind_typ U)] ++ E) ->
   wf_typ_in (F ++ [(x, bind_typ U)] ++ E) T ->
-  cv E U C ->
-  wf_typ_in (map (subst_cb x C) F ++ E) (subst_ct x C T).
+  wf_typ_in (map (subst_cb x (cv U)) F ++ E) (subst_ct x (cv U) T).
 Proof with eauto*.
-  intros * Hwf HwfT Hcv.
-  pose proof (cv_regular _ _ _ Hcv) as [_ [_ _]].
+  intros * Hwf HwfT.
   unfold wf_typ_in.
   erewrite dom_x_subst_away...
   eapply wf_typ_subst_cb...
   1, 2: simpl_env in *; apply wf_cset_extra...
-  apply ok_from_wf_env...
-  eapply wf_env_subst_cb...
 Qed.
 
-Lemma wf_pretyp_in_subst_cb_cv : forall U F E x C T,
+Lemma wf_pretyp_in_subst_cb_cv : forall U F E x T,
   wf_env (F ++ [(x, bind_typ U)] ++ E) ->
   wf_pretyp_in (F ++ [(x, bind_typ U)] ++ E) T ->
-  cv E U C ->
-  wf_pretyp_in (map (subst_cb x C) F ++ E) (subst_cpt x C T).
+  wf_pretyp_in (map (subst_cb x (cv U)) F ++ E) (subst_cpt x (cv U) T).
 Proof with eauto*.
-  intros * Hwf HwfT Hcv.
-  pose proof (cv_regular _ _ _ Hcv) as [_ [_ _]].
+  intros * Hwf HwfT.
   unfold wf_pretyp_in.
   erewrite dom_x_subst_away...
   eapply wf_pretyp_subst_cb...
   1, 2: simpl_env in *; apply wf_cset_extra...
-  apply ok_from_wf_env...
-  eapply wf_env_subst_cb...
 Qed.
 
-Lemma wf_typ_subst_cb_cv : forall U G F E x C T Ap Am,
+Lemma wf_typ_subst_cb_cv : forall U G F E x T Ap Am,
   wf_env (G ++ F ++ [(x, bind_typ U)] ++ E) ->
   wf_typ (G ++ F ++ [(x, bind_typ U)] ++ E) Ap Am T ->
-  cv E U C ->
   (dom E `union` dom F) `subset` Ap ->
   (dom E `union` dom F) `subset` Am ->
-  wf_typ (map (subst_cb x C) (G ++ F) ++ E) (Ap `remove` x) (Am `remove` x) (subst_ct x C T).
+  wf_typ (map (subst_cb x (cv U)) (G ++ F) ++ E) (Ap `remove` x) (Am `remove` x) (subst_ct x (cv U) T).
 Proof with eauto*.
-  intros * Hwf HwfT Hcv Hp Hm.
-  pose proof (cv_regular _ _ _ Hcv) as [_ [_ ?]].
+  intros * Hwf HwfT Hp Hm.
   eapply wf_typ_subst_cb; simpl_env...
   1, 2: simpl_env in *; apply wf_cset_extra...
-  rewrite_env (map (subst_cb x C) (G ++ F) ++ E)...
+  rewrite_env (map (subst_cb x (cv U)) (G ++ F) ++ E)...
   apply ok_from_wf_env...
   eapply wf_env_subst_cb...
   simpl_env in *...
 Qed.
 
-Lemma wf_pretyp_subst_cb_cv : forall U G F E x C T Ap Am,
+Lemma wf_pretyp_subst_cb_cv : forall U G F E x T Ap Am,
   wf_env (G ++ F ++ [(x, bind_typ U)] ++ E) ->
   wf_pretyp (G ++ F ++ [(x, bind_typ U)] ++ E) Ap Am T ->
-  cv E U C ->
   (dom E `union` dom F) `subset` Ap ->
   (dom E `union` dom F) `subset` Am ->
-  wf_pretyp (map (subst_cb x C) (G ++ F) ++ E) (Ap `remove` x) (Am `remove` x) (subst_cpt x C T).
+  wf_pretyp (map (subst_cb x (cv U)) (G ++ F) ++ E)
+            (Ap `remove` x)
+            (Am `remove` x)
+            (subst_cpt x (cv U) T).
 Proof with eauto*.
-  intros * Hwf HwfT Hcv Hp Hm.
-  pose proof (cv_regular _ _ _ Hcv) as [_ [_ _]].
+  intros * Hwf HwfT Hp Hm.
   eapply wf_pretyp_subst_cb; simpl_env...
   1, 2: simpl_env in *; apply wf_cset_extra...
-  rewrite_env (map (subst_cb x C) (G ++ F) ++ E)...
+  rewrite_env (map (subst_cb x (cv U)) (G ++ F) ++ E)...
   apply ok_from_wf_env...
   eapply wf_env_subst_cb...
   simpl_env in *...
 Qed.
-
-Ltac destruct_set_mem a bs :=
-  match type of bs with
-  | AtomSet.F.t =>
-    let H := fresh a "In" in
-    destruct (AtomSet.F.mem a bs) eqn:H; rewrite_set_facts_in H
-  | NatSet.F.t =>
-    let H := fresh a "In" in
-    destruct (NatSet.F.mem a bs) eqn:H; rewrite_set_facts_in H
-  end.
-
-Lemma cv_strengthen : forall F E T C,
-  wf_env (F ++ E) ->
-  wf_typ_in E T ->
-  cv (F ++ E) T C ->
-  cv E T C.
-Proof with eauto.
-  intros * WfE WfT Cv.
-  induction F...
-  destruct a as (Y & B).
-  simpl_env in *.
-  forwards: cv_unique_shrink_head Cv...
-  rewrite_env (empty ++ F ++ E).
-  eapply wf_typ_weakening.
-  1: apply WfT.
-  2,3: trivial...
-  apply ok_from_wf_env in WfE...
-Qed.
-
 
 Lemma binds_unique : forall b1 b2 x (E : env),
   binds x b1 E ->
@@ -731,165 +424,230 @@ Proof.
   congruence.
 Qed.
 
+Ltac note00 T id tac :=
+  assert (T) as id by tac;
+  inversion id;
+  subst.
+
+Lemma wf_typ_in_weakening : forall T E F G,
+  wf_typ_in (G ++ E) T ->
+  ok (G ++ F ++ E) ->
+  wf_typ_in (G ++ F ++ E) T.
+Proof with eauto.
+  intros * Hwf Hok.
+  eapply wf_typ_weakening...
+Qed.
+
+Lemma wf_pretyp_in_weakening : forall T E F G,
+  wf_pretyp_in (G ++ E) T ->
+  ok (G ++ F ++ E) ->
+  wf_pretyp_in (G ++ F ++ E) T.
+Proof with eauto.
+  intros * Hwf Hok.
+  eapply wf_pretyp_weakening...
+Qed.
+
+Lemma wf_cset_in_weakening : forall E F G C,
+  wf_cset_in (G ++ E) C ->
+  ok (G ++ F ++ E) ->
+  wf_cset_in (G ++ F ++ E) C.
+Proof with eauto.
+  intros * Hwf Hok.
+  eapply wf_cset_weakening...
+Qed.
+
 (* Substituting the same capture set preserves subcapturing *)
-Lemma subcapt_through_subst_cset : forall F x U E C1 C2 D,
+Lemma subcapt_through_subst_cset : forall x U F E C1 C2 ,
   subcapt (F ++ [(x, bind_typ U)] ++ E) C1 C2 ->
   wf_env (F ++ [(x, bind_typ U)] ++ E) ->
-  cv E U D ->
-  subcapt (map (subst_cb x D) F ++ E) (subst_cset x D C1) (subst_cset x D C2).
+  subcapt (map (subst_cb x (cv U)) F ++ E) (subst_cset x (cv U) C1) (subst_cset x (cv U) C2).
 Proof with eauto using wf_env_subst_cb, wf_cset_subst_cb with fsetdec.
-  intros * Hsc WfE CvU.
+  intros * Hsc WfE.
   dependent induction Hsc.
-  - cbn [subst_cset cset_references_fvar_dec].
-    constructor...
-    apply (wf_cset_in_subst_cb U)...
-  - unfold subst_cset, cset_references_fvar_dec.
-    destruct_set_mem x (singleton x0).
+  - assert (wf_cset_in (map (subst_cb x (cv U)) F ++ E) (subst_cset x (cv U) C)) as ?WF. {
+      eapply wf_cset_in_subst_cb...
+    }
+    assert (wf_cset_in (map (subst_cb x (cv U)) F ++ E)
+                       (subst_cset x (cv U) (cset_set xs {}N true))) as ?WF. {
+      eapply wf_cset_in_subst_cb...
+    }
+    cbv [subst_cset] in *.
+    destruct_set_mem x xs.
+    + assert (wf_typ_in (F ++ [(x, bind_typ U)] ++ E) U) as HA. {
+        note00 (wf_env ([(x, bind_typ U)] ++ E)) ident:(id) ltac:(eauto)...
+        rewrite_env (empty ++ (F ++ [(x, bind_typ U)]) ++ E).
+        apply wf_typ_in_weakening; simpl_env...
+      }
+      forwards: cv_wf HA.
+      inversion HA; subst; unfold cset_union; csetsimpl.
+      * unfold cset_union in WF; csetsimpl.
+        apply subcapt_universal...
+        replace (cset_set ({X}A `u`A xs `\`A x) {}N true)
+          with ((`cset_fvar` X) `u` (cset_set (xs `\`A x) {}N true)) by csetdec.
+        apply wf_cset_union.
+        (* -- enough (wf_cset_in (map (subst_cb x (`cset_fvar` X)) F ++ E) (cv X))... *)
+        (*    apply wf_cset_in_subst_cb. *)
+        (* unfold wf_cset_in in H2. *)
+        (* 1: apply H2. *)
+        1,2: admit.             (* wf_cset *)
+      * inversion H2; subst.
+        apply subcapt_universal...
+        admit.                  (* wf_cset *)
+    + apply subcapt_universal...
+  - unfold subst_cset.
+    destruct_set_mem x {x0}A.
     + destruct_set_mem x xs.
       2: exfalso; fsetdec.
-      note (wf_cset_in E D).
-      1: simpl cset_union; constructor...
-      simpl cset_union.
-      rewrite elim_empty_nat_set.
+      assert (wf_cset_in (F ++ [(x, bind_typ U)] ++ E) (cv U)) as HA. {
+        note00 (wf_env ([(x, bind_typ U)] ++ E)) ident:(id) ltac:(eauto)...
+        rewrite_env (empty ++ (F ++ [(x, bind_typ U)]) ++ E).
+        apply wf_cset_in_weakening; simpl_env...
+      }
+      inversion HA; subst.
+      unfold cset_union; csetsimpl.
       replace (fvars `union` singleton x0 `remove` x) with fvars by fsetdec.
       apply subcapt_set...
-      1: admit.
-      intros y yIn.
-      apply subcapt_in...
-      1,2: admit.
+      * admit.                  (* wf_cset *)
+      * intros y yIn.
+        apply subcapt_in...
+        1,2: admit.             (* wf_cset *)
+      * csetdec.
     + destruct_set_mem x xs.
       2: {
         apply subcapt_in...
-        1,2: admit.
+        1,2: admit.             (* wf_cset *)
       }
-      note (wf_cset_in E D).
-      1: simpl; constructor...
-      1: admit.
-      simpl; rewrite elim_empty_nat_set.
+      assert (wf_cset_in (F ++ [(x, bind_typ U)] ++ E) (cv U)) as HA. {
+        note00 (wf_env ([(x, bind_typ U)] ++ E)) ident:(id) ltac:(eauto)...
+        rewrite_env (empty ++ (F ++ [(x, bind_typ U)]) ++ E).
+        apply wf_cset_in_weakening; simpl_env...
+      }
+      inversion HA; subst.
+      unfold cset_union; csetsimpl.
       apply subcapt_in...
-      1,2: admit.
-  - unfold subst_cset at 1, cset_references_fvar_dec.
+      1,2: admit.               (* wf_cset *)
+  - admit.                      (* annoying case analysis followed by subcapt_in_univ *)
+  - unfold subst_cset at 1.
     destruct_set_mem x (singleton x0).
     + assert (x0 = x) by fsetdec; subst.
       assert (binds x (bind_typ U) (F ++ [(x, bind_typ U)] ++ E)) as HA by auto.
       forwards EQ: binds_typ_unique H HA; subst; clear HA.
-      forwards: cv_through_subst_ct x U H0...
-      assert (wf_typ_in E U) by auto.
+      assert (wf_typ_in E U) by eauto.
       assert (x `notin` dom E) as HA. {
         assert (ok (F ++ [(x, bind_typ U)] ++ E)) as HA by auto.
         apply ok_tail in HA.
         inversion HA...
       }
-      forwards: notin_fv_wf_typ H2 HA.
-      rewrite <- subst_ct_fresh in H1.
-      2: fsetdec.
-      apply cv_strengthen in H1...
-      specialize (IHHsc F x U E ltac:(trivial) ltac:(trivial) ltac:(trivial)).
-      forwards EQ: cv_unique H1 CvU...
-      rewrite EQ in IHHsc.
-      simpl.
-      replace (singleton x `remove` x) with {}.
-      2: fsetdec.
-      replace (cset_union D _) with D.
-      2: destruct D; [simpl;auto|cset_eq_dec].
-      trivial.
+      forwards: notin_fv_wf_typ H0 HA.
+      replace (cv U `u` cset_set ({x}A `\`A x) {}N false)
+              with (cv U) by (destruct U; csetdec).
+      replace (cv U) with (subst_cset x (cv U) (cv U)) at 2.
+      2: {
+        symmetry.
+        apply subst_cset_fresh.
+        destruct U; simpl in *; try fsetdec.
+      }
+      eapply IHHsc...
     + assert (x0 <> x) by fsetdec.
       binds_cases H.
-      * specialize (IHHsc F x U E ltac:(trivial) ltac:(trivial) ltac:(trivial)).
+      * specialize (IHHsc x U F E ltac:(trivial) ltac:(trivial)).
         forwards: wf_typ_from_binds_typ H...
-        assert (cv E T C) as HA. {
-          rewrite_env ((F ++ [(x, bind_typ U)]) ++ E) in H0.
-          forwards: cv_strengthen H0; simpl_env...
+        eapply subcapt_var with (T := T)...
+        replace (cv T) with (subst_cset x (cv U) (cv T)).
+        2: {
+          symmetry; apply subst_cset_fresh.
+          assert (x `notin` dom E) as HA. {
+            assert (ok (F ++ [(x, bind_typ U)] ++ E)) as HA by auto.
+            apply ok_tail in HA.
+            inversion HA...
+          }
+          forwards: notin_fv_wf_typ H1 HA.
+          destruct T; simpl in *; fsetdec.
         }
-        assert (x `notin` dom E) as HA'. {
-          assert (ok (F ++ [(x, bind_typ U)] ++ E)) as HA' by auto.
-          apply ok_tail in HA'.
-          inversion HA'...
+        apply IHHsc...
+      * assert (binds x0 (bind_typ (subst_ct x (cv U) T)) (map (subst_cb x (cv U)) F ++ E)) as HBnd by auto.
+        eapply subcapt_var...
+        replace (cv (subst_ct x (cv U) T))
+          with (subst_cset x (cv U) (cv T)).
+        2: {
+          destruct T; simpl...
+          - unfold subst_cset.
+            destruct_if...
+            exfalso;csetdec.
+          - (* x is bound as a term var, therefore `x <> a`. Needs a lemma. *)
+            admit.
         }
-        note (wf_cset_in E C).
-        1: {
-          inversion Hsc; subst.
-          unfold subst_cset, cset_references_fvar_dec.
-          constructor...
-          forwards: binds_In H.
-          constructor.
-          2: simpl_env...
-          intros y yIn.
-          rewrite AtomSetFacts.singleton_iff in yIn; symmetry in yIn; subst...
+        apply IHHsc...
+  - unfold subst_cset at 1.
+    destruct_set_mem x (singleton x0).
+    + assert (x0 = x) by fsetdec; subst.
+      assert (binds x (bind_typ U) (F ++ [(x, bind_typ U)] ++ E)) as HA by auto.
+      forwards EQ: binds_unique H HA.
+      exfalso;congruence.
+    + assert (x0 <> x) by fsetdec.
+      binds_cases H.
+      * specialize (IHHsc x U F E ltac:(trivial) ltac:(trivial)).
+        forwards: wf_typ_from_binds_sub H...
+        eapply subcapt_tvar with (T := T)...
+        replace (cv T) with (subst_cset x (cv U) (cv T)).
+        2: {
+          symmetry; apply subst_cset_fresh.
+          assert (x `notin` dom E) as HA. {
+            assert (ok (F ++ [(x, bind_typ U)] ++ E)) as HA by auto.
+            apply ok_tail in HA.
+            inversion HA...
+          }
+          forwards: notin_fv_wf_typ H1 HA.
+          destruct T; simpl in *; fsetdec.
         }
-        assert (x `notin` fvars) by fsetdec.
-        eapply subcapt_var with (T := T) (C := (cset_set fvars {}N)).
-        1: rewrite <- nil_concat; apply binds_weaken; simpl_env...
-        1: rewrite_env (empty ++ map (subst_cb x D) F ++ E); eapply cv_weakening; simpl_env...
-        unfold subst_cset at 1, cset_references_fvar_dec in IHHsc.
-        destruct_set_mem x fvars; [exfalso;fsetdec|].
-        trivial.
-      * assert (binds x0 (bind_typ (subst_ct x D T)) (map (subst_cb x D) F ++ E)) as HBnd by auto.
-        forwards Cv__post: cv_through_subst_ct H0...
-  - unfold subst_cset at 1, cset_references_fvar_dec.
+        apply IHHsc...
+      * assert (binds x0 (bind_sub (subst_ct x (cv U) T)) (map (subst_cb x (cv U)) F ++ E)) as HBnd by auto.
+        eapply subcapt_tvar...
+        replace (cv (subst_ct x (cv U) T))
+          with (subst_cset x (cv U) (cv T)).
+        2: {
+          destruct T; simpl...
+          - unfold subst_cset.
+            destruct_if...
+            exfalso;csetdec.
+          - (* x is bound as a term var, therefore `x <> a`. Needs a lemma. *)
+            admit.
+        }
+        apply IHHsc...
+  - unfold subst_cset at 1.
     destruct_set_mem x xs.
     2: {
       apply subcapt_set.
       1: admit.               (* wf_cset *)
+      2: {
+        (* Should we have a lemma that `cset_uvar` is not affected by subst? *)
+        (* Looking at that chain, we probably should. *)
+        destruct D; unfold subst_cset; destruct_if; destruct U; csetdec.
+      }
       intros y yIn.
-      replace (cset_set (singleton y) {}N)
-        with (subst_cset x D (cset_set (singleton y) {}N))...
-      unfold subst_cset, cset_references_fvar_dec.
-      destruct_set_mem x (singleton y); (trivial||exfalso;fsetdec).
+      replace (`cset_fvar` y) with (subst_cset x (cv U) (`cset_fvar` y))...
+      unfold subst_cset.
+      destruct_set_mem x (singleton y)...
+      exfalso;fsetdec.
     }
 
-    unfold AtomSet.F.For_all in H1.
+    unfold AtomSet.F.For_all in H0.
 
-    note (wf_cset_in E D). {
-      simpl.
-      specialize (H0 x xIn).
-      simpl in H0; simpl_env in H0.
-      dependent induction H0.
-      - unfold subst_cset, cset_references_fvar_dec.
-        constructor...
-      - Local Ltac cleanup_singleton_eq x y x0 x1 :=
-          let HA := fresh "HA" in
-          let xEQ := fresh x "EQ" in
-          rename x into xEQ;
-          rename x1 into x;
-          assert (x0 `in` singleton x0) as HA by fsetdec;
-          rewrite xEQ in HA;
-          assert (x0 = y) by fsetdec;
-          subst;
-          clear xEQ HA.
-        cleanup_singleton_eq x x x0 x1.
-
-        unfold subst_cset, cset_references_fvar_dec.
-        destruct_set_mem x xs0; [|exfalso;fsetdec]...
-      - cleanup_singleton_eq x x x0 x1.
-        replace T with U in *.
-        2: {
-          assert (binds x (bind_typ U) (F ++ [(x, bind_typ U)] ++ E)) as HBnd by auto.
-          forwards: binds_unique HBnd H2.
-          congruence.
-        }
-        replace C with cset_universal in *.
-        2: {
-          rewrite_env ((F ++ [(x, bind_typ U)]) ++ E) in H0.
-          apply cv_strengthen in H0...
-          forwards: cv_unique H0 CvU; simpl_env...
-        }
-        inversion H1...
-      - eapply H1...
+    inversion H; subst.
+    assert (wf_cset_in (F ++ [(x, bind_typ U)] ++ E) (cv U)) as HA. {
+      note00 (wf_env ([(x, bind_typ U)] ++ E)) ident:(id) ltac:(eauto)...
+      rewrite_env (empty ++ (F ++ [(x, bind_typ U)]) ++ E).
+      apply wf_cset_in_weakening; simpl_env...
     }
-    note (wf_cset_in (F ++ [(x, bind_typ U)] ++ E) D0). {
-      unfold subst_cset, cset_references_fvar_dec.
-      constructor...
-      admit.                    (* wf_cset *)
-    }
+    inversion HA; subst.
 
-    rename fvars into ds.
-    rename fvars0 into cs'.
-    unfold subst_cset, cset_references_fvar_dec.
+    rename fvars into cs', univ into b__c', fvars0 into ds, univ0 into b__d.
+    unfold subst_cset.
     destruct_set_mem x cs'.
-    + simpl; rewrite elim_empty_nat_set.
+    + unfold cset_union; csetsimpl.
       apply subcapt_set.
       1: admit.               (* wf_cset *)
+      2: csetdec.
       intros y yIn.
       Ltac destruct_union_mem H :=
         rewrite AtomSetFacts.union_iff in H; destruct H.
@@ -899,71 +657,153 @@ Proof with eauto using wf_env_subst_cb, wf_cset_subst_cb with fsetdec.
       }
 
       specialize (H0 y ltac:(fsetdec)); simpl in H0.
+      Local Ltac cleanup_singleton_eq x y x0 x1 :=
+        let HA := fresh "HA" in
+        let xEQ := fresh x "EQ" in
+        rename x into xEQ;
+        rename x1 into x;
+        assert (x0 `in` singleton x0) as HA by fsetdec;
+        rewrite xEQ in HA;
+        assert (x0 = y) by fsetdec;
+        subst;
+        clear xEQ HA.
 
       dependent induction H0.
+      * csetsimpl.
+        apply subcapt_universal.
+        1,2: admit.             (* wf_cset *)
       * cleanup_singleton_eq x y x0 x1.
         apply subcapt_in...
         1,2: admit.             (* wf_cset *)
       * cleanup_singleton_eq x y x0 x1.
-        replace (cset_set (singleton y) {}N)
-          with (subst_cset x (cset_set ds {}N) (cset_set (singleton y) {}N)).
+        rename select (_ = cv U) into EQ.
+        replace (`cset_fvar` y) with (subst_cset x (cv U) (`cset_fvar` y)).
         2: {
-          unfold subst_cset, cset_references_fvar_dec; simpl.
+          unfold subst_cset; simpl.
           destruct_set_mem x (singleton y); (trivial || exfalso;fsetdec).
         }
-        replace (cset_set (ds `union` cs' `remove` x) {}N)
-          with (subst_cset x (cset_set ds {}N) (cset_set cs' {}N)).
+        replace (cset_set (ds `union` cs' `remove` x) {}N (b__d || b__c'))
+          with (subst_cset x (cv U) (cset_set cs' {}N b__c')).
         2: {
-          unfold subst_cset, cset_references_fvar_dec; simpl.
+          unfold subst_cset; simpl.
           destruct_set_mem x cs'; [|exfalso;fsetdec].
-          simpl; rewrite elim_empty_nat_set.
-          trivial.
+          rewrite <- EQ.
+          unfold cset_union; csetsimpl.
         }
-        eapply H3...
-      * eapply H1...
-    + simpl; rewrite elim_empty_nat_set.
+        rewrite EQ.
+        eapply H1...
+      * cleanup_singleton_eq x y x0 x1.
+        rename select (_ = cv U) into EQ.
+        replace (`cset_fvar` y) with (subst_cset x (cv U) (`cset_fvar` y)).
+        2: {
+          unfold subst_cset; simpl.
+          destruct_set_mem x (singleton y); (trivial || exfalso;fsetdec).
+        }
+        replace (cset_set (ds `union` cs' `remove` x) {}N (b__d || b__c'))
+          with (subst_cset x (cv U) (cset_set cs' {}N b__c')).
+        2: {
+          unfold subst_cset; simpl.
+          destruct_set_mem x cs'; [|exfalso;fsetdec].
+          rewrite <- EQ.
+          unfold cset_union; csetsimpl.
+        }
+        rewrite EQ.
+        eapply H1...
+      * rename select (_ = cv U) into EQ.
+        replace (`cset_fvar` y) with (subst_cset x (cv U) (`cset_fvar` y)).
+        2: {
+          unfold subst_cset; simpl.
+          destruct_set_mem x (singleton y); (trivial || exfalso;fsetdec).
+        }
+        replace (cset_set (ds `union` cs' `remove` x) {}N (b__d || b__c'))
+          with (subst_cset x (cv U) (cset_set cs' {}N b__c')).
+        2: {
+          unfold subst_cset; simpl.
+          destruct_set_mem x cs'; [|exfalso;fsetdec].
+          rewrite <- EQ.
+          unfold cset_union; csetsimpl.
+        }
+        rewrite EQ.
+        eapply H1...
+    + unfold cset_union; csetsimpl.
+      rename select (_ = cv U) into EQ.
       apply subcapt_set.
       1: admit.                (* wf_cset *)
+      2: {
+        all: destr_bool.
+        admit.                  (* undoable as-is, we must know more about the set relationship *)
+      }
       intros y yIn.
       destruct_set_mem y (xs `remove` x).
       * specialize (H0 y ltac:(fsetdec)); simpl in H0.
         dependent induction H0.
+        -- apply subcapt_universal.
+           1,2: admit.             (* wf_cset *)
         -- cleanup_singleton_eq x y x0 x1.
            apply subcapt_in...
            1,2: admit.             (* wf_cset *)
         -- cleanup_singleton_eq x y x0 x1.
-           replace (cset_set (singleton y) {}N)
-             with (subst_cset x (cset_set ds {}N) (cset_set (singleton y) {}N)).
+           replace (`cset_fvar` y)
+             with (subst_cset x (cv U) (`cset_fvar` y)).
            2: {
-             unfold subst_cset, cset_references_fvar_dec; simpl.
-             destruct_set_mem x (singleton y); (trivial || exfalso;fsetdec).
+             unfold subst_cset; simpl.
+             destruct_set_mem x (`cset_fvar` y); (trivial || exfalso;fsetdec).
            }
-           replace (cset_set cs' {}N)
-             with (subst_cset x (cset_set ds {}N) (cset_set cs' {}N)).
+           replace (cset_set cs' {}N b__c')
+             with (subst_cset x (cv U) (cset_set cs' {}N b__c')).
            2: {
-             unfold subst_cset, cset_references_fvar_dec; simpl.
+             unfold subst_cset; simpl.
              destruct_set_mem x cs'; (trivial||exfalso;fsetdec).
            }
-           eapply H3...
-        -- eapply H1...
+           rewrite EQ.
+           eapply H1...
+        -- cleanup_singleton_eq x y x0 x1.
+           replace (`cset_fvar` y)
+             with (subst_cset x (cv U) (`cset_fvar` y)).
+           2: {
+             unfold subst_cset; simpl.
+             destruct_set_mem x (`cset_fvar` y); (trivial || exfalso;fsetdec).
+           }
+           replace (cset_set cs' {}N b__c')
+             with (subst_cset x (cv U) (cset_set cs' {}N b__c')).
+           2: {
+             unfold subst_cset; simpl.
+             destruct_set_mem x cs'; (trivial||exfalso;fsetdec).
+           }
+           rewrite EQ.
+           eapply H1...
+        -- replace (`cset_fvar` y) with (subst_cset x (cv U) (`cset_fvar` y)).
+           2: {
+             unfold subst_cset; simpl.
+             destruct_set_mem x (`cset_fvar` y); (trivial || exfalso;fsetdec).
+           }
+           replace (cset_set cs' {}N b__c') with (subst_cset x (cv U) (cset_set cs' {}N b__c')).
+           2: {
+             unfold subst_cset; simpl.
+             destruct_set_mem x cs'; (trivial||exfalso;fsetdec).
+           }
+           rewrite EQ.
+           eapply H1...
       * destruct_union_mem yIn.
         2: exfalso...
-        specialize (H1 x xIn _ _ _ _ ltac:(reflexivity) ltac:(trivial) ltac:(trivial)).
-        unfold subst_cset at 1, cset_references_fvar_dec in H1.
-        destruct_set_mem x (singleton x); [|exfalso;fsetdec].
+        specialize (H1 x xIn _ _ _ _ ltac:(reflexivity) ltac:(trivial)).
+        admit.
+        (* unfold subst_cset at 1 in H1. *)
+        (* destruct_set_mem x (singleton x); [|exfalso;fsetdec]. *)
 
-        unfold subst_cset at 1, cset_references_fvar_dec in H1.
-        destruct_set_mem x cs'; [exfalso;fsetdec|].
+        (* unfold subst_cset at 1 in H1. *)
+        (* destruct_set_mem x cs'; [exfalso;fsetdec|]. *)
 
-        simpl in H1; rewrite elim_empty_nat_set in H1.
+        (* unfold cset_union in H1 *)
+        (* simpl in H1; csetsimpl in H1. *)
 
-        replace (ds `union` singleton x `remove` x) with ds in H1 by fsetdec.
+        (* replace (ds `union` singleton x `remove` x) with ds in H1 by fsetdec. *)
 
-        enough (subcapt (map (subst_cb x (cset_set ds {}N)) F ++ E)
-                         (cset_set (singleton y) {}N)
-                         (cset_set ds {}N)) as HA. {
-          eapply subcapt_transitivity...
-        }
-        eapply subcapt_in...
-        admit.             (* wf_cset *)
+        (* enough (subcapt (map (subst_cb x (cset_set ds {}N)) F ++ E) *)
+        (*                  (cset_set (singleton y) {}N) *)
+        (*                  (cset_set ds {}N)) as HA. { *)
+        (*   eapply subcapt_transitivity... *)
+        (* } *)
+        (* eapply subcapt_in... *)
+        (* admit.             (* wf_cset *) *)
 Admitted.
